nola/iris/proph.v
@@ -3,13 +3,13 @@
 From nola.util Require Export proph.
 From nola.iris Require Export upd.
 From nola.util Require Import rel plist.
-From nola.iris Require Import discrete_fun.
-From iris.algebra Require Import auth functions gmap csum frac agree.
+From nola.iris Require Import list gmap.
+From iris.algebra Require Import gmap csum frac agree.
 From iris.bi Require Import fractional.
 From iris.proofmode Require Import proofmode.
 Import EqNotations.
 
-Implicit Type TY : synty.
+Implicit Type (TY : synty) (q : Qp).
 
 (** ** Prophecy log *)
 
@@ -30,6 +30,11 @@ Local Definition proph_log TY := list (proph_log_item TY).
 (** Prophecy variables of a prophecy log *)
 Local Definition pl_vars {TY} (L : proph_log TY) : list (aprvar TY) :=
   pli_var <$> L.
+(** Prophecy ids of a prophecy log *)
+Local Definition pl_ids {TY} (L : proph_log TY) : gset positive :=
+  list_to_set ((λ ξ, aprvar_id ξ) <$> pl_vars L).
+
+(** Prophecy log item in a prophecy log *)
 
 (** Prophecy dependency over the complement of a list set *)
 Local Definition proph_dep_out {TY A}
@@ -42,7 +47,7 @@ Local Notation "aπ ./~ ξl" := (proph_dep_out aπ ξl)
 Local Fixpoint proph_log_valid {TY} (L : proph_log TY) :=
   match L with
   | [] => True
-  | .{ξ := aπ} :: L' => ξ ∉ pl_vars L' ∧ aπ ./~ pl_vars L ∧ proph_log_valid L'
+  | .{ξ := xπ} :: L' => ξ ∉ pl_vars L' ∧ xπ ./~ pl_vars L ∧ proph_log_valid L'
   end.
 Local Notation ".✓ L" := (proph_log_valid L) (at level 20, format ".✓  L").
 
@@ -53,30 +58,30 @@ Local Notation "π ◁ L" := (proph_sat π L) (at level 70, format "π  ◁  L")
 
 (** A prophecy assignment updated at a prophecy variable *)
 Local Definition proph_upd {TY}
-  (ξ : aprvar TY) (aπ : proph_asn TY → ξ.(aprvar_ty)) π : proph_asn TY := λ η,
+  (ξ : aprvar TY) (xπ : proph_asn TY → ξ.(aprvar_ty)) π : proph_asn TY := λ η,
   match decide (ξ = η) with
-  | left eq => rew[aprvar_ty] eq in aπ π
+  | left eq => rew[aprvar_ty] eq in xπ π
   | right _ => π η
   end.
-Local Notation ":<[ ξ := aπ ]>" := (proph_upd ξ aπ)
-  (at level 5, format ":<[ ξ  :=  aπ ]>").
+Local Notation ":<[ ξ := xπ ]>" := (proph_upd ξ xπ)
+  (at level 5, format ":<[ ξ  :=  xπ ]>").
 
 (** Access on [proph_upd] *)
-Local Lemma proph_upd_self {TY} {π : proph_asn TY} {ξ aπ} :
-  :<[ξ := aπ]> π ξ = aπ π.
+Local Lemma proph_upd_self {TY} {π : proph_asn TY} {ξ xπ} :
+  :<[ξ := xπ]> π ξ = xπ π.
 Proof.
-  rewrite /proph_upd. case: (decide (ξ = ξ)); [|done]=> eq.
+  unfold proph_upd. case: (decide (ξ = ξ)); [|done]=> eq.
   by rewrite (eq_dec_refl eq).
 Qed.
-Local Lemma proph_upd_ne {TY} {π : proph_asn TY} {ξ aπ η} :
-  ξ ≠ η → :<[ξ := aπ]> π η = π η.
-Proof. rewrite /proph_upd. by case (decide (ξ = η)). Qed.
+Local Lemma proph_upd_ne {TY} {π : proph_asn TY} {ξ xπ η} :
+  ξ ≠ η → :<[ξ := xπ]> π η = π η.
+Proof. unfold proph_upd. by case (decide (ξ = η)). Qed.
 
 (** Prophecy assignment updated by a prophecy log *)
 Local Fixpoint proph_upds {TY} L (π : proph_asn TY) :=
   match L with
   | [] => π
-  | .{ξ := aπ} :: L' => proph_upds L' (:<[ξ := aπ]> π)
+  | .{ξ := xπ} :: L' => proph_upds L' (:<[ξ := xπ]> π)
   end.
 Local Notation ":<[ L ]>" := (proph_upds L) (at level 5, format ":<[ L ]>").
 
@@ -92,10 +97,10 @@ Qed.
 Local Lemma proph_valid_upds_sat {TY} {L : proph_log TY} :
   .✓ L → ∀ π, :<[L]> π ◁ L.
 Proof.
-  rewrite /proph_sat. elim: L=>/= [|[ξ aπ] L' IH]; [done|].
+  rewrite /proph_sat. elim: L=>/= [|[ξ xπ] L' IH]; [done|].
   move=> [?[? /IH ?]]?. apply Forall_cons=>/=. split; [|done].
   rewrite proph_upds_eqv_out; [|done]. rewrite proph_upd_self.
-  set L := .{ξ := aπ} :: L'. have dep': aπ ./~ pl_vars L by done. symmetry.
+  set L := .{ξ := xπ} :: L'. have dep': xπ ./~ pl_vars L by done. symmetry.
   apply dep', (proph_upds_eqv_out L).
 Qed.
 (** [L] can by satisfied for valid [L] *)
@@ -105,17 +110,160 @@ Proof. exists (:<[L]> inhabitant). by apply proph_valid_upds_sat. Qed.
 (** ** Prophecy resource algebra *)
 
 (** Algebra for a prophecy variable *)
-Local Definition proph_itemR {TY} (X : TY) :=
-  csumR fracR (agreeR (leibnizO (proph_asn TY → X))).
-(** Algebra for prophecy variables of a type *)
-Local Definition proph_gmapR {TY} (X : TY) := gmapR positive (proph_itemR X).
-(** Algebra for all prophecy variables *)
-Local Definition proph_smryR TY := discrete_funR (proph_gmapR (TY:=TY)).
-(** Algebra for the prophecy machinery *)
-Local Definition prophR_def TY := authR (proph_smryR TY).
-Lemma prophR_aux : seal prophR_def. Proof. by eexists. Qed.
+Local Definition proph_aitemR TY :=
+  agreeR (leibnizO (anyty TY (λ A, proph_asn TY → A))).
+Local Definition proph_itemR TY := csumR fracR (proph_aitemR TY).
+(** Base algebra for the prophecy machinery *)
+Local Definition proph_mapR TY := gmapR positive (proph_itemR TY).
+
+(** Carrier of the algebra for the prophecy machinery *)
+#[projections(primitive)]
+Record proph_car TY := ProphCar { un_proph_car : proph_mapR TY }.
+Arguments ProphCar {_}. Arguments un_proph_car {_}.
+Add Printing Constructor proph_car.
+
+(** Equivalence *)
+Local Instance proph_equiv_instance {TY} : Equiv (proph_car TY) :=
+  λ '(ProphCar M) '(ProphCar M'), M ≡ M'.
+Local Lemma proph_equiv {TY a a'} :
+  (a ≡ a') = (a.(un_proph_car (TY:=TY)) ≡ a'.(un_proph_car)).
+Proof. done. Qed.
+
+(** Discrete [ofe] structure *)
+Local Instance proph_equivalence {TY} : Equivalence (≡@{proph_car TY}).
+Proof. split=> >; apply ofe_equivalence. Qed.
+#[warnings="-redundant-canonical-projection"]
+Local Canonical prophO TY := discreteO (proph_car TY).
+
+(** [ProphCar] and [un_proph_car] are proper *)
+Local Instance Proph_proper {TY} :
+  Proper ((≡) ==> (≡)) (ProphCar (TY:=TY)).
+Proof. solve_proper. Qed.
+Local Instance unproph_proper {TY} :
+  Proper ((≡) ==> (≡)) (un_proph_car (TY:=TY)).
+Proof. solve_proper. Qed.
+
+(** Core *)
+Local Instance proph_pcore_instance {TY} : PCore (proph_car TY) :=
+  λ '(ProphCar M), ProphCar <$> pcore M.
+Local Lemma proph_pcore {TY a} :
+  pcore a = ProphCar (TY:=TY) <$> pcore a.(un_proph_car).
+Proof. done. Qed.
+
+(** Operation *)
+Local Instance proph_op_instance {TY} : Op (proph_car TY) :=
+  λ '(ProphCar M) '(ProphCar M'), ProphCar (M ⋅ M').
+Local Lemma proph_op {TY a a'} :
+  a ⋅ a' = ProphCar (TY:=TY) (a.(un_proph_car) ⋅ a'.(un_proph_car)).
+Proof. done. Qed.
+Local Lemma proph_included {TY a a'} :
+  a ≼ a' ↔ a.(un_proph_car (TY:=TY)) ≼ a'.(un_proph_car).
+Proof.
+  unfold included=>/=. split.
+  { move=> [[M]]. by exists M. } { move=> [M]. by exists (ProphCar M). }
+Qed.
+
+(** Fractional item *)
+Local Definition fitem {TY} q : proph_itemR TY := Cinl q.
+(** Agreement item *)
+Local Definition aitem {TY X} xπ : proph_itemR TY :=
+  Cinr (to_agree (Anyty X xπ)).
+
+(** A prophecy map simulating a prophecy log *)
+Local Definition proph_sim {TY} (M : proph_mapR TY) L :=
+  (∀ ξ,
+    (∃ q, M !! aprvar_id ξ ≡ Some (fitem q)) → ξ ∉ pl_vars L) ∧
+  (∀ ξ xπ, M !! aprvar_id ξ ≡ Some (aitem xπ) → .{ξ := xπ} ∈ L).
+Local Notation "M :~ L" := (proph_sim M L) (at level 70, format "M  :~  L").
+
+(** [proph_sim] is proper *)
+Local Instance proph_sim_proper {TY} :
+  Proper ((≡) ==> (=) ==> iff) (proph_sim (TY:=TY)).
+Proof.
+  have H (M M' : proph_mapR TY) L : M ≡ M' → M :~ L → M' :~ L; last first.
+  { move=> ?? eq ??<-. split; by apply H. }
+  move=> eq [sim sim']. split.
+  - move=> ?[q eq']. apply sim. exists q. by rewrite -eq'.
+  - move=> ?? eq'. apply sim'. by rewrite -eq'.
+Qed.
+
+(** [proph_sim] is antitone over inclusion *)
+Local Lemma proph_sim_op_l {TY M M'} {L : proph_log TY} :
+  ✓ (M ⋅ M') → M ⋅ M' :~ L → M :~ L.
+Proof.
+  move=> val [sim sim']. split.
+  - move=> ξ [q eq]. apply sim. move: (val ξ.(prvar_id)).
+    rewrite lookup_op. setoid_rewrite eq.
+    case: (M' !! ξ.(prvar_id)); last first.
+    { move=> _. exists q. by rewrite right_id. }
+    case; [|done..]=> q' _. by exists (q + q')%Qp.
+  - move=> ξ xπ eq. apply sim'. move: (val ξ.(prvar_id)).
+    rewrite lookup_op. setoid_rewrite eq.
+    case: (M' !! ξ.(prvar_id)); [|by rewrite right_id].
+    case; [done| |done]=> b /agree_op_inv <-.
+    apply Some_proper, (Cinr_proper (B:=proph_aitemR TY)), agree_idemp.
+Qed.
+Local Lemma proph_sim_op_r {TY M M'} {L : proph_log TY} :
+  ✓ (M ⋅ M') → M ⋅ M' :~ L → M' :~ L.
+Proof. rewrite comm. exact proph_sim_op_l. Qed.
+
+(** Validity *)
+Local Instance proph_valid_instance {TY} : Valid (proph_car TY) :=
+  λ '(ProphCar M), ✓ M ∧ ∃ L, M :~ L ∧ .✓ L.
+Local Lemma proph_valid {TY a} :
+  (✓ a) = (✓ a.(un_proph_car (TY:=TY)) ∧ ∃ L, a.(un_proph_car) :~ L ∧ .✓ L).
+Proof. done. Qed.
+
+(** Discrete [cmra] structure *)
+Local Lemma proph_ra_mixin TY : RAMixin (proph_car TY).
+Proof.
+  split.
+  - move=> ???. rewrite !proph_equiv. solve_proper.
+  - move=> [?][?][?]. rewrite !proph_equiv !proph_pcore /=.
+    move=> eq [<-]. eexists _. split; [done|]. solve_proper.
+  - move=> [?][?]. rewrite proph_equiv !proph_valid /==> eq.
+    f_equiv. { by rewrite eq. } do 3 f_equiv. by rewrite eq.
+  - move=> [?][?][?]. rewrite !proph_op proph_equiv /=. apply assoc, _.
+  - move=> [?][?]. rewrite !proph_op proph_equiv /=. apply comm, _.
+  - move=> [?][?]. rewrite proph_pcore proph_op proph_equiv /==> [=<-].
+    apply (cmra_core_l (A:=proph_mapR TY)).
+  - move=> [?][?]. rewrite !proph_pcore /==> [=<-]. do 2 f_equiv.
+    apply (cmra_core_idemp (A:=proph_mapR TY)).
+  - move=> [M][M'][?]. rewrite proph_included proph_pcore /==> inc [=<-].
+    exists (ProphCar (omap pcore M')). rewrite proph_included proph_pcore /=.
+    split; [done|]. exact (cmra_core_mono _ _ inc).
+  - move=> [M][M']. rewrite proph_op !proph_valid /=.
+    move=> [val[L[[sim sim'] ?]]]. split. { by eapply cmra_valid_op_l. }
+    exists L. split; [|done]. by eapply proph_sim_op_l.
+Qed.
+#[warnings="-redundant-canonical-projection"]
+Local Canonical prophR_def TY : cmra :=
+  discreteR (proph_car TY) (proph_ra_mixin TY).
+Local Lemma prophR_aux : seal prophR_def. Proof. by eexists. Qed.
 Definition prophR := prophR_aux.(unseal).
-Lemma prophR_unseal : prophR = prophR_def. Proof. exact: seal_eq. Qed.
+Local Lemma prophR_unseal : prophR = prophR_def. Proof. exact: seal_eq. Qed.
+Local Instance prophR_discrete {TY} : CmraDiscrete (prophR_def TY).
+Proof. apply discrete_cmra_discrete. Qed.
+
+(** Unit *)
+Local Instance proph_unit_instance {TY} : Unit (proph_car TY) := ProphCar ∅.
+Local Lemma proph_unit {TY} : ε = ProphCar (TY:=TY) ∅. Proof. done. Qed.
+
+(** [ucmra] structure *)
+Local Lemma proph_ucmra_mixin TY : UcmraMixin (proph_car TY).
+Proof.
+  split.
+  - split; [done|]. exists []. split; [|done].
+    split; [move=> ?[?+]|move=> ??]; rewrite lookup_empty=> eq;
+      by apply symmetry, None_equiv_eq in eq.
+  - move=> [?]. by rewrite proph_unit proph_op proph_equiv /= left_id.
+  - done.
+Qed.
+#[warnings="-redundant-canonical-projection"]
+Local Canonical prophUR TY : ucmra :=
+  Ucmra (proph_car TY) (proph_ucmra_mixin TY).
+Local Instance prophR_total {TY} : CmraTotal (prophR_def TY).
+Proof. exact (cmra_unit_cmra_total (A:=prophUR TY)). Qed.
 
 (** Ghost state *)
 Class prophGS TY Σ := ProphGS {
@@ -132,94 +280,29 @@ Definition prophΣ TY := GFunctor (prophR TY).
 #[export] Instance subG_prophPreG `{!subG (prophΣ TY) Σ} : prophGpreS TY Σ.
 Proof. solve_inG. Qed.
 
-(** Access a summary at a prophecy variable *)
-Local Notation "S .!! ξ" := (S ξ.(aprvar_ty) !! ξ.(aprvar_var).(prvar_id))
-  (at level 20, format "S  .!!  ξ").
-
-(** Fractional item *)
-Local Definition fitem {TY} {X : TY} (q : Qp) : proph_itemR X := Cinl q.
-(** Agreement item *)
-Local Definition aitem {TY} {X : TY} aπ : proph_itemR X := Cinr (to_agree aπ).
-(** One line in a prophecy summary *)
-Local Definition line {TY} ξ it : proph_smryR TY :=
-  .{[ξ.(aprvar_ty) := {[ξ.(prvar_id) := it]}]}.
-(** Add a line in a prophecy summary *)
-Local Definition add_line {TY} ξ it (S : proph_smryR TY) : proph_smryR TY :=
-  .<[ξ.(aprvar_ty) := <[ξ.(prvar_id) := it]> (S ξ.(aprvar_ty))]> S.
-
-(** Access [add_line] out of the additionn *)
-Local Lemma add_line_ne {TY} {ξ η : aprvar TY} {S aπ} : ξ ≠ η →
-  add_line ξ (aitem aπ) S .!! η = S .!! η.
-Proof.
-  move: aπ. case: ξ η=> [X[h i]][Y[h' j]] ? ne.
-  rewrite /add_line /discrete_fun_insert /=.
-  case (decide (X = Y)); [|done]=> eq. simplify_eq=>/=.
-  case (decide (i = j))=> ?; [|by rewrite lookup_insert_ne]. simplify_eq.
-  move: ne. by rewrite (proof_irrel h h').
-Qed.
-
-(** A prophecy summary simulating a prophecy log *)
-Local Definition proph_sim {TY} (S : proph_smryR TY) (L : proph_log TY) :=
-  ∀ (ξ : aprvar _) aπ, S .!! ξ ≡ Some (aitem aπ) ↔ .{ξ := aπ} ∈ L.
-Local Notation "S :~ L" := (proph_sim S L) (at level 70, format "S  :~  L").
-
-(** [:~] on [add_line] *)
-Local Lemma add_line_fitem_sim {TY} {S : proph_smryR TY} {L} {ξ} :
-  S :~ L → S .!! ξ = None → add_line ξ (fitem 1) S :~ L.
-Proof.
-  move: ξ=> [X[? i]] sim no [Y[? j]]?.
-  rewrite -sim /add_line /discrete_fun_insert /=.
-  case: (decide (X = Y)); [|done]=> ?. subst=>/=.
-  case: (decide (i = j))=> ?; [|by rewrite lookup_insert_ne]. subst.
-  rewrite lookup_insert no.
-  split=> eqv; [apply (inj Some) in eqv|]; inversion eqv.
-Qed.
-Local Lemma add_line_aitem_sim {TY} {S : proph_smryR TY} {L ξ aπ} :
-  S :~ L → ξ ∉ pl_vars L → add_line ξ (aitem aπ) S :~ .{ξ := aπ} :: L.
-Proof.
-  move=> sim ?. have inLne η wπ : .{η := wπ} ∈ L → ξ ≠ η.
-  { move=> /(elem_of_list_fmap_1 pli_var) ??. by subst. }
-  move=> η bπ. rewrite elem_of_cons. case (decide (ξ = η))=> ?.
-  { subst. rewrite /add_line discrete_fun_lookup_insert lookup_insert. split.
-    - move=> /(inj (Some ∘ aitem)) ->. by left.
-    - move=> [[?]|/inLne ?]; by [simplify_eq|]. }
-  rewrite add_line_ne; [|done]. rewrite sim. split; [by right|].
-  case; [|done]=> ?. simplify_eq.
-Qed.
-
 (** ** Iris propositions *)
 
 Section defs.
   Context `{!prophGS TY Σ}.
+  Implicit Type (X : TY) (pli : proph_log_item TY).
 
   (** Prophecy token *)
-  Local Definition proph_tok_def (ξ : aprvar _) (q : Qp) : iProp Σ :=
-    own proph_name (◯ line ξ (fitem q)).
+  Local Definition proph_tok_def (ξ : aprvar TY) q : iProp Σ :=
+    own proph_name (ProphCar {[ξ.(prvar_id) := fitem q]}).
   Lemma proph_tok_aux : seal proph_tok_def. Proof. by eexists. Qed.
   Definition proph_tok := proph_tok_aux.(unseal).
   Lemma proph_tok_unseal : proph_tok = proph_tok_def.
   Proof. exact: seal_eq. Qed.
 
   (** Atomic prophecy observation *)
-  Local Definition proph_aobs pli : iProp Σ :=
-    own proph_name (◯ line pli.(pli_var) (aitem pli.(pli_val))).
+  Local Definition proph_aobs pli : iProp Σ := own proph_name
+    (ProphCar {[pli.(pli_var).(prvar_id) := aitem pli.(pli_val)]}).
   (** Prophecy observation *)
   Local Definition proph_obs_def (φπ : proph_asn TY → Prop) : iProp Σ :=
-    ∃L, ⌜∀ π, π ◁ L → φπ π⌝ ∗ [∗ list] pli ∈ L, proph_aobs pli.
+    ∃ L, ⌜∀ π, π ◁ L → φπ π⌝ ∗ [∗ list] pli ∈ L, proph_aobs pli.
   Lemma proph_obs_aux : seal proph_obs_def. Proof. by eexists. Qed.
   Definition proph_obs := proph_obs_aux.(unseal).
   Lemma proph_obs_unseal : proph_obs = proph_obs_def.
-  Proof. exact: seal_eq. Qed.
-
-  (** Token for a prophecy summary *)
-  Local Definition proph_smry_tok (S : proph_smryR TY) : iProp Σ :=
-    own proph_name (● S).
-  (** World satisfaction for the prophecy *)
-  Local Definition proph_wsat_def : iProp Σ :=
-    ∃ S, ⌜∃L, .✓ L ∧ S :~ L⌝ ∗ proph_smry_tok S.
-  Lemma proph_wsat_aux : seal proph_wsat_def. Proof. by eexists. Qed.
-  Definition proph_wsat := proph_wsat_aux.(unseal).
-  Lemma proph_wsat_unseal : proph_wsat = proph_wsat_def.
   Proof. exact: seal_eq. Qed.
 End defs.
 
@@ -235,27 +318,25 @@ Notation "⟨ π , φ ⟩" := (proph_obs (λ π, φ%type%stdpp))
 
 (** ** Lemmas *)
 
-(** Allocate [proph_wsat] *)
-Lemma proph_wsat_alloc `{!prophGpreS TY Σ} :
-  ⊢ |==> ∃ _ : prophGS TY Σ, proph_wsat.
+(** Initialize [prophGS] *)
+Lemma proph_init `{!prophGpreS TY Σ} :
+  ⊢ |==> ∃ _ : prophGS TY Σ, True : iProp Σ.
 Proof.
-  iMod (own_alloc (● ε)) as (γ) "●"; [by apply auth_auth_valid|]. iModIntro.
-  iExists (ProphGS _ _ _ γ). rewrite proph_wsat_unseal.
-  iExists ε. iFrame "●". iPureIntro. exists []. split; [done|]=> ??.
-  rewrite lookup_empty. split=> hyp; inversion hyp.
+  iMod (own_alloc (ε : prophR_def TY)) as (γ) "_".
+  { exact ucmra_unit_valid. } { by iExists (ProphGS _ _ _ γ). }
 Qed.
 
 Section lemmas.
   Context `{!prophGS TY Σ}.
-  Implicit Type (φπ ψπ : proph_asn TY → Prop).
+  Implicit Type (X : TY) (φπ ψπ : proph_asn TY → Prop) (ψ : Prop).
 
   (** [proph_tok] is timelesss and fractional *)
   #[export] Instance proph_tok_timeless {q ξ} : Timeless q:[ξ].
   Proof. rewrite proph_tok_unseal. exact _. Qed.
   #[export] Instance proph_tok_fractional {ξ} : Fractional (λ q, q:[ξ]%I).
   Proof.
-    move=> ??. by rewrite proph_tok_unseal -own_op -auth_frag_op
-      discrete_fun_singleton_op singleton_op -Cinl_op.
+    move=> ??.
+    by rewrite proph_tok_unseal -own_op proph_op singleton_op -Cinl_op.
   Qed.
   #[export] Instance proph_tok_as_fractional {q ξ} :
     AsFractional q:[ξ] (λ q, q:[ξ]%I) q.
@@ -283,6 +364,11 @@ Section lemmas.
   Qed.
 
   (** [proph_obs] is persistent, timeless and monotone *)
+  Local Instance proph_aobs_persistent {pli} : Persistent (proph_aobs pli).
+  Proof.
+    apply own_core_persistent. rewrite /CoreId proph_pcore /=. do 2 f_equiv.
+    by apply singleton_core'.
+  Qed.
   #[export] Instance proph_obs_persistent {φπ} : Persistent .⟨φπ⟩.
   Proof. rewrite proph_obs_unseal. exact _. Qed.
   #[export] Instance proph_obs_timeless {φπ} : Timeless .⟨φπ⟩.
@@ -323,129 +409,167 @@ Section lemmas.
     do 2 f_equiv. move=> [??]. by apply imp.
   Qed.
 
-  (** [proph_wsat] is timeless *)
-  #[export] Instance proph_wsat_timeless : Timeless proph_wsat.
-  Proof. rewrite proph_wsat_unseal. exact _. Qed.
-
-  (** Lemma for [proph_alloc] *)
-  Local Lemma proph_alloc' {S} (ξ : aprvar TY) : S .!! ξ = None →
-    proph_smry_tok S ==∗ proph_smry_tok (add_line ξ (fitem 1) S) ∗ 1:[ξ].
+  (** Update of [proph_alloc] *)
+  Local Lemma proph_alloc_upd :
+    ε ~~>: (λ a : prophR_def TY, ∃ i, a = ProphCar {[i := fitem 1]}).
   Proof.
-    rewrite proph_tok_unseal=> ?. iIntros "●".
-    iMod (own_update with "●") as "[$$]"; [|done].
-    by apply auth_update_alloc,
-      discrete_fun_insert_local_update, alloc_singleton_local_update.
+    apply cmra_total_updateP. setoid_rewrite <-cmra_discrete_valid_iff=> _ [M].
+    rewrite left_id /=. move=> [val[L[[sim sim'] ?]]].
+    set i := fresh (dom M ∪ pl_ids L). exists (ProphCar {[i := fitem 1]}).
+    split; [by eexists _|]. split=>/=.
+    - move=> j. rewrite lookup_op. case: (decide (j = i)).
+      + move=> ->. rewrite lookup_singleton. have ->: M !! i = None; [|done].
+        apply (not_elem_of_dom M), (not_elem_of_union _ _ (pl_ids L)), is_fresh.
+      + move=> ?. rewrite lookup_singleton_ne; [|done]. by rewrite left_id.
+    - exists L. split; [|done]. split.
+      + move=> ξ [q +]. rewrite lookup_op. case: (decide (ξ.(prvar_id) = i)).
+        * move=> eq _ /(elem_of_list_fmap_1 (λ ξ, aprvar_id ξ)). rewrite eq.
+          eapply (not_elem_of_list_to_set (C:=gset _) i (_ <$> _)), proj2,
+            not_elem_of_union, is_fresh.
+        * move=> ?. rewrite lookup_singleton_ne; [|done]. rewrite left_id=> ?.
+          apply sim. by exists q.
+      + move=> ξ ?. rewrite lookup_op. case: (decide (ξ.(prvar_id) = i)).
+        * move=> ->. rewrite lookup_singleton.
+          case: (M !! i)=>/=; [case=> > eq|move=> eq]; apply (inj Some) in eq;
+            inversion eq.
+        * move=> ?. rewrite lookup_singleton_ne; [|done]. rewrite left_id.
+          apply sim'.
   Qed.
   (** Allocate a new prophecy variable *)
-  Lemma proph_alloc {X : TY} : X → ⊢ |=[proph_wsat]=> ∃ ξ : prvar X, 1:[ξ].
+  Lemma proph_alloc {X} : X → ⊢ |==> ∃ ξ : prvar X, 1:[ξ].
   Proof.
-    rewrite proph_wsat_unseal=> x. iIntros "[%S [[%L[% %sim]] ●]]".
-    set ξ := Prvar (synty_to_inhab x) (fresh (dom (S X))).
-    have ?: S .!! ξ = None. { apply (not_elem_of_dom_1 (S X)), is_fresh. }
-    iMod (proph_alloc' ξ with "●") as "[● ξ]"; [done|]. iModIntro.
-    iSplitL "●"; [|iExists _; by iFrame]. iExists _. iFrame "●". iPureIntro.
-    exists L. split; by [|apply add_line_fitem_sim].
+    move=> x. iMod (own_unit (prophUR TY) proph_name) as "ε".
+    iMod (own_updateP with "ε") as "big"; [apply proph_alloc_upd|].
+    iDestruct "big" as (?[i->]) "?". iExists (Prvar (synty_to_inhab x) i).
+    by rewrite proph_tok_unseal.
   Qed.
   (** Allocate new prophecy variables *)
   Lemma proph_alloc_list {Xl} : plist synty_ty Xl →
-    ⊢ |=[proph_wsat]=> ∃ ξl : plist _ Xl, 1:∗[of_plist_prvar ξl].
+    ⊢ |==> ∃ ξl : plist _ Xl, 1:∗[of_plist_prvar ξl].
   Proof.
     elim: Xl; [move=>/= ?; by iExists ()|]=>/= ?? IH [x xl].
     iMod (IH xl) as (ξl) "ξl". iMod (proph_alloc x) as (ξ) "ξ".
     iModIntro. iExists (ξ, ξl)'. iFrame.
   Qed.
 
-  (** Lemmas for [proph_resolve_dep] *)
-  Local Lemma proph_tok_out {S L ξ q} :
-    S :~ L → proph_smry_tok S -∗ q:[ξ] -∗ ⌜ξ ∉ pl_vars L⌝.
+  (** Simplify [[^op list]] over [ProphCar] *)
+  Local Lemma big_cmra_opL_Proph {A al} (F : A → proph_mapR TY) :
+    un_proph_car ([^op list] a ∈ al, ProphCar (F a)) ≡ ([^op list] a ∈ al, F a).
+  Proof. by elim: al=>/=; [done|]=> ?? ->. Qed.
+
+  (** Lemmas for [proph_resolve_dep_upd] *)
+  Local Lemma aitem_no_fitem {X xπ q o} :
+    Some (aitem (X:=X) xπ) ⋅ o ≡ Some (fitem q) → False.
   Proof.
-    rewrite proph_tok_unseal=> sim. iIntros "● ξ".
-    iDestruct (own_valid_2 with "● ξ") as %val. iPureIntro.
-    move=> /(elem_of_list_fmap_2 pli_var) [[[X ?]?][? /sim eqv]]. simpl in *.
-    subst. move: val=> /auth_both_valid_discrete[inc _].
-    move/(discrete_fun_included_spec_1 _ _ X) in inc.
-    rewrite /line discrete_fun_lookup_singleton /= in inc. move: eqv.
-    move: inc=> /singleton_included_l[?[-> inc]] eqv. apply (inj Some) in eqv.
-    move: inc. by rewrite eqv=> /Some_csum_included [|[[?[?[_[?]]]]|[?[?[?]]]]].
+    move=> eq. have: Some (aitem xπ) ≼ Some (fitem q) by eexists _.
+    move=> /Some_included[eq'|[it +]]; [inversion eq'|].
+    case it=> > eq'; inversion eq'.
   Qed.
-  Local Lemma proph_tok_ne {ξ η q} : 1:[ξ] -∗ q:[η] -∗ ⌜ξ ≠ η⌝.
+  Local Lemma aitem_eq_agree {X xπ Y yπ o} :
+    Some (aitem xπ) ⋅ o ≡ Some (aitem yπ) →
+    Anyty (F:=λ A, _ → A) X xπ = Anyty Y yπ.
   Proof.
-    rewrite proph_tok_unseal. iIntros "ξ η".
-    iDestruct (own_valid_2 with "ξ η") as %val. iPureIntro=> ?. subst.
-    move: val. rewrite -auth_frag_op auth_frag_valid discrete_fun_singleton_op
-      discrete_fun_singleton_valid singleton_op singleton_valid -Cinl_op
-      Cinl_valid.
-    apply exclusive_l, _.
+    move=> eq. have: Some (aitem xπ) ≼ Some (aitem yπ) by eexists _.
+    move=> /Some_included[/Cinr_inj/to_agree_inj ?|[it ?]]; [done|].
+    have: aitem xπ ≼ aitem yπ by eexists _.
+    by move=> /Cinr_included/to_agree_included ?.
   Qed.
-  Local Lemma proph_resolve_obs {S ξ aπ} :
-    proph_smry_tok S -∗ 1:[ξ] ==∗
-      proph_smry_tok (add_line ξ (aitem aπ) S) ∗ ⟨π, π ξ = aπ π⟩.
+  (** Update of [proph_resolve_dep] *)
+  Local Lemma proph_resolve_dep_upd {ηl ξ xπ q} : xπ ./ ηl →
+    ProphCar {[aprvar_id ξ := fitem (TY:=TY) 1]} ⋅
+    ([^op list] η ∈ ηl, ProphCar {[aprvar_id η := fitem q]}) ~~>
+      ProphCar {[aprvar_id .{ξ := xπ}.(pli_var) := aitem .{ξ := xπ}.(pli_val)]} ⋅
+      ([^op list] η ∈ ηl, ProphCar {[aprvar_id η := fitem q]}).
   Proof.
-    rewrite proph_tok_unseal. iIntros "● ξ".
-    iMod (own_update_2 with "● ξ") as "[$ ?]".
-    { apply auth_update, discrete_fun_singleton_local_update_any,
-        singleton_local_update_any=> ? _.
-      by apply exclusive_local_update. }
-    iModIntro. rewrite proph_obs_unseal. iExists [.{ξ := aπ}].
-    rewrite big_sepL_singleton. iSplitR; [|done]. iPureIntro=> ? sat.
-    by inversion sat.
+    move=> dep. apply cmra_total_update.
+    setoid_rewrite <-cmra_discrete_valid_iff=> _ [M].
+    rewrite !proph_valid /=. move=> [val[L[sim ?]]]. split.
+    { have: {[ξ.(prvar_id) := fitem 1]} ~~> {[ξ.(prvar_id) := aitem xπ]}
+        by apply singleton_update, cmra_update_exclusive.
+      move=> /cmra_total_update. setoid_rewrite <-cmra_discrete_valid_iff.
+      move=> upd. move: val. rewrite -!assoc. apply upd, 0. }
+    exists (.{ξ := xπ} :: L)=>/=. split.
+    - move: val sim. rewrite -!assoc. move: (_ ⋅ M)=> M' val sim. split=>/=.
+      + move=> ζ [r eq]. apply not_elem_of_cons. split.
+        { move=> ?. subst. move: eq. rewrite lookup_op lookup_singleton.
+          apply aitem_no_fitem. }
+        apply sim. exists r. move: eq. rewrite !lookup_op.
+        case: (decide (ζ.(prvar_id) = ξ.(prvar_id))).
+        { move=> ->. by rewrite !lookup_singleton=> /aitem_no_fitem. }
+        move=> ?. rewrite !lookup_singleton_ne; [|done..].
+        by rewrite left_id=> ->.
+      + move=> ζ yπ eq. apply elem_of_cons.
+        case: (decide (ζ.(prvar_id) = ξ.(prvar_id))); last first.
+        { move=> ?. right. apply sim. move: eq. rewrite !lookup_op.
+          by rewrite !lookup_singleton_ne; [|done..]. }
+        move=> eqi. move: eq. rewrite eqi lookup_op lookup_singleton.
+        move=> /aitem_eq_agree. move: eqi. clear. move: xπ yπ.
+        have ->: ξ = Aprvar ξ.(aprvar_ty) ξ.(aprvar_var); [done|].
+        have ->: ζ = Aprvar ζ.(aprvar_ty) ζ.(aprvar_var); [done|].
+        move: (ξ.(aprvar_ty)) (ξ.(aprvar_var)) (ζ.(aprvar_ty))
+          (ζ.(aprvar_var))=> ?[h ?]?[h' ?]/=??.
+        left. simplify_eq. by rewrite (proof_irrel h h').
+    - apply (proph_sim_op_l val) in sim. apply cmra_valid_op_l in val.
+      split; [|split; [|done]].
+      { apply (proph_sim_op_l val) in sim. apply sim. exists 1%Qp.
+        by rewrite lookup_singleton. }
+      move=> ?? eqπ. apply dep=> η el. apply eqπ. apply not_elem_of_cons.
+      move: val sim. rewrite big_cmra_opL_Proph.
+      case: (big_cmra_opL_elem_of (C:=proph_mapR TY)
+        (λ η, {[aprvar_id η := fitem q]}) el)=> [?->].
+      rewrite assoc=> val /(proph_sim_op_l val) sim.
+      apply cmra_valid_op_l in val. split.
+      + move=> ?. subst. move: (val ξ.(prvar_id)). clear.
+        rewrite lookup_op !lookup_singleton Some_valid Cinl_valid frac_valid.
+        by eapply Qp.not_add_le_l.
+      + apply (proph_sim_op_r val) in sim. apply sim. exists q.
+        by rewrite lookup_singleton.
   Qed.
   (** Resolve a prophecy *)
-  Lemma proph_resolve_dep ηl ξ aπ q : aπ ./ ηl →
-    1:[ξ] -∗ q:∗[ηl] =[proph_wsat]=∗ q:∗[ηl] ∗ ⟨π, π ξ = aπ π⟩.
+  Lemma proph_resolve_dep ηl ξ xπ q : xπ ./ ηl →
+    1:[ξ] -∗ q:∗[ηl] ==∗ q:∗[ηl] ∗ ⟨π, π ξ = xπ π⟩.
   Proof.
-    rewrite proph_wsat_unseal. iIntros (dep) "ξ ηl [%S[[%L[% %sim]] ●]]".
-    iDestruct (proph_tok_out with "● ξ") as %?; [done|].
-    set L' := .{ξ := aπ} :: L.
-    iAssert ⌜∀η, η ∈ ηl → η ∉ pl_vars L'⌝%I as %outηl.
-    { iIntros (? el).
-      iDestruct (big_sepL_elem_of with "ηl") as "η"; [apply el|].
-      iDestruct (proph_tok_ne with "ξ η") as %?.
-      iDestruct (proph_tok_out with "● η") as %?; [done|].
-      by rewrite not_elem_of_cons. }
-    iFrame "ηl". iMod (proph_resolve_obs with "● ξ") as "[● $]". iModIntro.
-    iExists _. iFrame "●". iPureIntro. exists L'.
-    split; [|by apply add_line_aitem_sim].
-    split; [done|split; [|done]]=> ?? eqv. apply dep=> ? /outηl ?. by apply eqv.
+    iIntros (dep) "ξ ηl". rewrite proph_tok_unseal.
+    iMod (to_own_big_cmra_opL with "ηl") as "ηl". iCombine "ξ ηl" as "ξηl".
+    iMod (own_update with "ξηl") as "big"; [apply (proph_resolve_dep_upd dep)|].
+    iModIntro. iDestruct "big" as "[aobs ηl]". rewrite of_own_big_cmra_opL.
+    iFrame "ηl". rewrite proph_obs_unseal. iExists [.{ξ := xπ}]. iFrame "aobs".
+    iSplit; [|done]. by iPureIntro=> ? /Forall_singleton.
   Qed.
-  Lemma proph_resolve ξ x : 1:[ξ] =[proph_wsat]=∗ ⟨π, π ξ = x⟩.
+  Lemma proph_resolve ξ x : 1:[ξ] ==∗ ⟨π, π ξ = x⟩.
   Proof.
     iIntros "ξ".
     by iMod (proph_resolve_dep [] ξ (λ _, x) 1 with "ξ [//]") as "[_ $]".
   Qed.
 
-  (** Lemma for [proph_obs_sat] *)
-  Local Lemma proph_aobs_agree {S ξ aπ} :
-    proph_smry_tok S -∗ proph_aobs .{ξ := aπ} -∗ ⌜S .!! ξ ≡ Some (aitem aπ)⌝.
+  (** Get [proph_sat] out of [✓] over [aitem]s *)
+  Local Lemma aitems_sat {L : proph_log TY} :
+    ✓ ([^op list] pli ∈ L,
+      ProphCar {[aprvar_id pli.(pli_var) := aitem pli.(pli_val)]}) →
+    ∃ π, π ◁ L.
   Proof.
-    iIntros "● a". iDestruct (own_valid_2 with "● a") as %val. iPureIntro.
-    move: val=> /auth_both_valid_discrete [inc val].
-    move/(discrete_fun_included_spec_1 _ _ ξ.(aprvar_ty)) in inc.
-    rewrite /line discrete_fun_lookup_singleton in inc.
-    move: inc=> /singleton_included_l[it[eqv /Some_included[->|inc]]]; [done|].
-    rewrite eqv. constructor.
-    apply (lookup_valid_Some _ ξ.(prvar_id) it) in val; [|done]. move: val.
-    move: inc=> /csum_included [->|[[?[?[?]]]|[?[?[eq[->inc]]]]]]; [done..|].
-    move=> val. move: inc. move: val=> /Cinr_valid/to_agree_uninj [?<-].
-    inversion eq. by move/to_agree_included <-.
+    move=> [val [L'[sim /proph_valid_sat[π /Forall_forall sat]]]]. exists π.
+    apply Forall_forall. move=> [ξ xπ] el. apply sat, sim.
+    move: (val ξ.(prvar_id)). rewrite big_cmra_opL_Proph.
+    case: (big_cmra_opL_elem_of (C:=proph_mapR TY) (λ pli,
+      {[aprvar_id pli.(pli_var) := aitem pli.(pli_val)]}) el)=> [M ->]=>/=.
+    rewrite lookup_op lookup_singleton.
+    case: (M !! ξ.(prvar_id)); [|by rewrite right_id]. case; [done| |done].
+    move=> ? /Some_valid/Cinr_valid val'. apply Some_proper.
+    apply (Cinr_proper (B:=proph_aitemR TY)). symmetry.
+    by apply agree_valid_included.
   Qed.
   (** Get a satisfiability from a prophecy observation *)
-  Lemma proph_obs_sat {φπ} : .⟨φπ⟩ =[proph_wsat]=∗ ⌜∃ π, φπ π⌝.
+  Lemma proph_obs_sat {φπ} : .⟨φπ⟩ ⊢ ⌜∃ π, φπ π⌝.
   Proof.
-    rewrite proph_wsat_unseal proph_obs_unseal.
-    iIntros "[%L'[%Toφπ #L']] [%S[[%L[%Lval %sim]] ●]]".
-    move: (Lval)=> /proph_valid_sat[π /Forall_forall sat]. iModIntro.
-    iAssert ⌜π ◁ L'⌝%I as %?; last first.
-    { iSplitL; last first. { iPureIntro. exists π. by apply Toφπ. }
-      iExists _. iFrame "●". iPureIntro. by exists L. }
-    rewrite /proph_sat Forall_forall. iIntros ([ξ aπ] el)=>/=.
-    iDestruct (proph_aobs_agree with "● []") as %eqv.
-    { by iApply big_sepL_elem_of. }
-    { iPureIntro. by apply (sat .{ξ := aπ}), sim. }
+    rewrite proph_obs_unseal. iDestruct 1 as (L to) "aobss".
+    iMod (to_own_big_cmra_opL with "aobss") as "aitems".
+    iDestruct (own_valid with "aitems") as %val. iPureIntro.
+    move: val=> /aitems_sat[π sat]. exists π. by apply to.
   Qed.
-  Lemma proph_obs_false {φπ} : (∀ π, ¬ φπ π) → .⟨φπ⟩ =[proph_wsat]=∗ False.
+  Lemma proph_obs_elim {φπ ψ} : (∀ π, φπ π → ψ) → .⟨φπ⟩ ⊢ ⌜ψ⌝.
   Proof.
-    iIntros (neg) "obs". iMod (proph_obs_sat with "obs") as %[? φx].
-    by apply neg in φx.
+    iIntros (to) "obs". iDestruct (proph_obs_sat with "obs") as %[? φx].
+    by apply to in φx.
   Qed.
 End lemmas.
