nola/iris/gmap.v
@@ -55,6 +55,11 @@ End map_with.
 Section gmapR.
   Context `{!EqDecision K, !Countable K} {C : cmra}.
 
+  (** [lookup] is proper *)
+  #[export] Instance lookup_proper i :
+    Proper ((≡@{gmapR K C}) ==> (≡@{optionR C})) (lookup i).
+  Proof. apply ne_proper, _. Qed.
+
   (** [singletonM] is proper *)
   #[export] Instance singleton_proper {i : K} :
     Proper ((≡@{C}) ==> (≡@{gmapR K C})) (singletonM i).
