nola/iris/list.v
@@ -1,7 +1,37 @@
 (** * Utility on [list] *)
 
 From nola Require Export prelude.
+From iris.algebra Require Import cmra.
+From iris.base_logic Require Import own.
 From iris.proofmode Require Import proofmode.
+
+(** ** On [[^op list]] *)
+Section big_cmra_opL.
+  Context {C : ucmra}.
+
+  (** For [∈] *)
+  Lemma big_cmra_opL_elem_of {A} {a al} (f : A → C) :
+    a ∈ al → f a ≼ [^op list] a ∈ al, f a.
+  Proof.
+    elim: al=>/=. { by move=> /elem_of_nil. }
+    move=> ?? IH /elem_of_cons[<-|/IH ?]; [done|]. by etrans.
+  Qed.
+
+  (** [own] on [[^op list]] *)
+  Lemma own_big_cmra_opL_as `{!inG Σ C} {A} {γ al} (f : A → C) :
+    own γ ([^op list] a ∈ al, f a) ⊣⊢
+      own γ ε ∗ [∗ list] a ∈ al, own γ (f a).
+  Proof.
+    elim: al=>/=; [by rewrite right_id|]=> ?? IH. rewrite own_op IH !assoc.
+    f_equiv. by rewrite comm.
+  Qed.
+  Lemma of_own_big_cmra_opL `{!inG Σ C} {A} {γ al} (f : A → C) :
+    own γ ([^op list] a ∈ al, f a) ⊢ [∗ list] a ∈ al, own γ (f a).
+  Proof. rewrite own_big_cmra_opL_as. by iIntros "[_$]". Qed.
+  Lemma to_own_big_cmra_opL `{!inG Σ C} {A} {γ al} (f : A → C) :
+    ([∗ list] a ∈ al, own γ (f a)) ⊢ |==> own γ ([^op list] a ∈ al, f a).
+  Proof. rewrite own_big_cmra_opL_as. iMod own_unit as "$". by iIntros. Qed.
+End big_cmra_opL.
 
 (** ** On [[∗ list]] *)
 Section big_sepL.
